# Exercises

## Paths

Give a value to the variables `answer` so that the following code can be
executed without typing errors.

The idea is that these constellations represent paths to complete in order to
obtain only the constellation `$ok` as a result.

```
checker = galaxy
  interaction: {test} {tested}.
  expect: $ok.
end
empty = {}.

answer = {replace_me}.
exercise1 :: empty [checker].
exercise1 = ((-1 $ok) {1})[1=>answer].

answer = {replace_me}.
exercise2 :: empty [checker].
exercise2 = ((-1; +2) {1})[1=>answer].

answer = {replace_me}.
exercise3 :: empty [checker].
exercise3 = ((-1 $ok; -2 +3) {1})[1=>answer].

answer = {replace_me}.
exercise4 :: empty [checker].
exercise4 = ((-f(+g(X)) $ok) {1})[1=>answer].

answer = {replace_me}.
exercise5 :: empty [checker].
exercise5 = ((+f($a) +f($b); +g($a); @+g($b) $ok) {1})[1=>answer].
```

<details>
  <summary>Solutions</summary>
<pre>
<code>

checker = galaxy
  interaction: {test} {tested}.
  expect: $ok.
end
empty = {}.

answer = +1.
exercise1 :: empty [checker]
exercise1 = ((-1 $ok) {1})[1=>answer].

answer = +1 -2 $ok.
exercise2 :: empty [checker]
exercise2 = ((-1; +2) {1})[1=>answer].

answer = +1 +2; -3.
exercise3 :: empty [checker]
exercise3 = ((-1 $ok; -2 +3) {1})[1=>answer].

answer = +f(-g(X)).
exercise4 :: empty [checker]
exercise4 = ((-f(+g(X)) $ok) {1})[1=>answer].

answer = -f($a); -f($b) -g($a) -g($b).
exercise5 :: empty [checker]
exercise5 = ((+f($a) +f($b); +g($a); @+g($b) $ok) {1})[1 => answer].

</code>
</pre>
</details>

## Dynamical registers

Start from the following program:

```
init = +r0($0).

print process
  init.
  {replace_me}.
end
```

representing a memory with a register `r0`.

Stellogen can represent memory but in a particular way, by destroying to
construct somewhere else. We cannot content ourselves of updating the register
with a star `-r0(X) +r0($1)` as this star has a circular dependency that would
allow it to be reused an unlimited number of times.

In fact, we can only move the register to modify it, for example with a star
`-r0($0) +r1($1)` that destroys the register `r0` and constructs a register
`r1` containing `$1`.

The goal is to define constellations. You can use the code above to do your
tests.

**Exercise 1.** Define two constellations allowing to update the register `r0`to `1` by using an intermediary star to save the value of `r0`.

<details>
  <summary>Solution</summary>
<pre>
<code>-r0(X) +tmp0(X).
-tmp0(X) +r0($1).
</code>
</pre>
</details>

**Exercise 2.** Define a constellation allowing to duplicate and move the register `r0` in two registers `r1` and `r2`.

<details>
  <summary>Solution</summary>
<pre>
<code>-r0(X) +r1(X);
-r0(X) +r2(X).
</code>
</pre>
</details>

**Exercise 3.** Define two constellations allowing to set the value of `r1` to `$0` then define two constellations allowing to exchange the values of `r1` and `r2`.

<details>
  <summary>Solution</summary>
<pre>
<code>-r1(X) +tmp0(X).
-tmp0(X) +r1($0).
-r1(X) +s1(X); -r2(X) +s2(X).
-s1(X) +r2(X); -s2(X) +r1(X).
</code>
</pre>
</details>

**Exercise 4.** How to duplicate `r1` so as to be able to follow and update its copies all at once (as if dealing with a single register) to the value `$5`?

<details>
  <summary>Solution</summary>
<pre>
<code>-r1(X) +r1($l X);
-r1(X) +r1($r X).
-r1(A X) +tmp0(A X).
-tmp0(A X) +r1(A $5).
</code>
</pre>
</details>

**Exercise 5.** Using the previous method, duplicate all copies at once.

<details>
  <summary>Solution</summary>
<pre>
<code>-r1(A X) +r1($l A X);
-r1(A X) +r1($r A X).
</code>
</pre>
</details>

## Boolean logic

We want to simulate boolean formulas with constellations. Each question uses
the result of the previous question.

**Exercise 1.** Define a constellation computing negation such that it yields `1` as output when added to the star `@-not($0 X) X` and `0` when added to `@-not($1 X) X`.

<details>
  <summary>Solution</summary>
<pre>
<code>not = +not($0 $1); +not($1 $0).
</code>
</pre>
</details>

**Exercise 2.** How to display the truth table of negation with a single star, such that we obtain the output `$table_not($0 $1); table_not($1 $0).`?

<details>
  <summary>Solution</summary>
<pre>
<code>print @-not(X Y) $table_not(X Y).
</code>
</pre>
</details>

**Exercise 3.** Write in two different ways constellations computing conjunction and disjunction and display their truth table in the same way as for the previous question.

<details>
  <summary>Solution</summary>
<pre>
<code>

and = +and($0 $0 $0); +and($0 $1 $0); +and($1 $0 $0); +and($1 $1 $1).
or  = +or($0 $0 $0); +or($0 $1 $1); +or($1 $0 $1); +or($1 $1 $1).

and2 = +and2($0 X $0); +and2($1 X X).
or2  = +or2($0 X X); +or2($1 X $1).

print @-and(X Y R) $table_and(X Y R).
print @-or(X Y R) $table_or(X Y R).
print @-and2(X Y R) $table_and2(X Y R).
print @-or2(X Y R) $table_or2(X Y R).

</code>
</pre>
</details>

**Exercise 4.** Use disjunction and negation to display the truth table of implication given that `X => Y = not(X) \/ Y`.

<details>
  <summary>Solution</summary>
<pre>
<code>

impl  = -not(X Y) -or(Y Z R) +impl(X Z R).
impl2 = -not(X Y) -or2(Y Z R) +impl2(X Z R).

print @-impl(X Y R) $table_impl(X Y R).
print @-impl2(X Y R) $table_impl2(X Y R).

</code>
</pre>
</details>

**Exercise 5.** Use implication and conjunction to display the truth table of logical equivalence given that `X <=> Y = (X => Y) /\ (X => Y)`.

<details>
  <summary>Solution</summary>
<pre>
<code>

eqq  = -impl(X Y R1) -impl(Y X R2) -and(R1 R2 R) +eqq(X Y R).
eqq2 = -impl2(X Y R1) -impl2(Y X R2) -and2(R1 R2 R) +eqq2(X Y R).

table_eqq  = @-eqq(X Y R) $table_eqq(X Y R).
table_eqq2 = @-eqq2(X Y R) $table_eqq2(X Y R).

</code>
</pre>
</details>

**Exercise 6.** Define a constellation representing the formula of exclded middle `X \/ ~X`. Display the truth table corresponding to this formula.

<details>
  <summary>Solution</summary>
<pre>
<code>

ex = -not(X R1) -or(R1 X R2) +ex(X R2).
print -ex(X R) $table_ex(X R).

</code>
</pre>
</details>

**Exercise 7.** Determine for which values of `X`, `Y` and `Z` the formula `X /\ ~(Y \/ Z)` is true.

<details>
  <summary>Solution</summary>
<pre>
<code>print -or(Y Z R1) -not(R1 R2) -and(X R2 1) $x(X) $y(Y) $z(Z).
</code>
</pre>
</details>
